Expand Lambda's basic functions to support arbitrary types rather than LMonoTy, fix broken Reflect (#211)
This patch expand Lambda's basic functions to support arbitrary types
rather than LMonoTy, to use them for formal evaluation semantics of
Lambda which should be agnostic of the type system.

This also fixes broken Reflect.

Also:

- Generalize Factory's two top-level fns to receive non LMonoTy as well
- Remove getConcreteLFuncCall because it must use isCanonicalValue, not
isConst, but isCanonicalValue cannot be used due to cyclic dependency
between modules .. and it isn't used anywhere.



By submitting this pull request, I confirm that you can use, modify,
copy, and redistribute this contribution, under the terms of your
choice.

Strata/DL/Lambda/Identifiers.lean
@@ -34,26 +34,26 @@ instance {IDMeta} [Inhabited IDMeta] : Coe String (Identifier IDMeta) where
   coe s := ⟨s, Inhabited.default⟩
 
 /--
-Identifiers, optionally with their inferred monotype.
+Identifiers, optionally with their inferred type.
 -/
-abbrev IdentT (IDMeta : Type) := (Identifier IDMeta) × Option LMonoTy
-abbrev IdentTs (IDMeta : Type) := List (IdentT IDMeta)
+abbrev IdentT (ITy IDMeta: Type) := (Identifier IDMeta) × Option ITy
+abbrev IdentTs (ITy IDMeta: Type) := List (IdentT ITy IDMeta)
 
-instance {IDMeta : Type} : ToFormat (IdentT IDMeta) where
+instance {IDMeta ITy: Type} [ToFormat ITy]: ToFormat (IdentT ITy IDMeta) where
   format i := match i.snd with
     | none => f!"{i.fst}"
     | some ty => f!"({i.fst} : {ty})"
 
-def IdentT.ident (x : (IdentT IDMeta)) : Identifier IDMeta :=
+def IdentT.ident (x : (IdentT ITy IDMeta)) : Identifier IDMeta :=
   x.fst
 
-def IdentT.monoty? (x : (IdentT IDMeta)) : Option LMonoTy :=
+def IdentT.ty? (x : (IdentT ITy IDMeta)) : Option ITy :=
   x.snd
 
-def IdentTs.idents (xs : (IdentTs IDMeta)) : List (Identifier IDMeta) :=
+def IdentTs.idents (xs : (IdentTs ITy IDMeta)) : List (Identifier IDMeta) :=
   xs.map Prod.fst
 
-def IdentTs.monotys? (xs : (IdentTs IDMeta)) : List (Option LMonoTy) :=
+def IdentTs.tys? (xs : (IdentTs ITy IDMeta)) : List (Option ITy) :=
   xs.map Prod.snd
 
 abbrev Identifiers IDMeta := Std.HashMap String IDMeta
