Strata/DL/Lambda/Lambda.lean
@@ -8,6 +8,7 @@ import Strata.DL.Lambda.LExprEval
 import Strata.DL.Lambda.LExprType
 import Strata.DL.Lambda.LExpr
 import Strata.DL.Lambda.TypeFactory
+import Strata.DL.Lambda.Reflect
 
 namespace Lambda
 
